

1. write the Maclaurin's series expansion.

If $f: [0, x] \rightarrow \mathbb{R}$ is such that

i). $f^{(n-1)}$ is continuous on $[0, x]$

ii). $f^{(n-1)}$ is derivable on $(0, x)$ and $p \in \mathbb{Z}^+$

then \exists a real number $\theta \in (0, 1)$ such that

$$f(x) = f(0) + x f'(0) + \frac{x^2}{2!} f''(0) + \dots + \frac{x^{n-1}}{(n-1)!} f^{(n-1)}(0) + \frac{x^n (1-\theta)^{n-p}}{p(n-1)!} f^{(n)}(\theta x).$$

2. If $u = x \sin y$, $v = y \sin x$ find $\frac{\partial(u, v)}{\partial(x, y)}$.

Sol: Given

$$u = x \sin y, \quad v = y \sin x$$

$$\frac{\partial u}{\partial x} = (1) \sin y$$

$$\frac{\partial v}{\partial x} = y \cos x$$

$$\frac{\partial u}{\partial y} = x \cos y$$

$$\frac{\partial v}{\partial y} = (1) \sin x$$

now,

$$\frac{\partial(u, v)}{\partial(x, y)} = \begin{vmatrix} \frac{\partial u}{\partial x} & \frac{\partial u}{\partial y} \\ \frac{\partial v}{\partial x} & \frac{\partial v}{\partial y} \end{vmatrix}$$

$$= \begin{vmatrix} \sin y & x \cos y \\ y \cos x & \sin x \end{vmatrix} = \sin x \cdot \sin y - x y \cos x \cos y //$$

3. write the Taylor's series expansion of two variables.

Ans: The Taylor series expansion for a function of two variables, $f(x, y)$ around a points $(x-a)$ & $(y-b)$ is

$$f(x, y) = f(a, b) + [(x-a)f_x(a, b) + (y-b)f_y(a, b)] +$$

$$\frac{1}{2!} [(x-a)^2 f_{xx}(a, b) + 2(x-a)(y-b) f_{xy}(a, b) + (y-b)^2 f_{yy}(a, b)] + \dots //$$

4. find $\Gamma\left(\frac{9}{2}\right)$.

Sol: To find $\Gamma\left(\frac{9}{2}\right)$

we know that $\Gamma(n) = (n-1)\Gamma(n-1)$

put $n = \frac{9}{2}$

$$\therefore \Gamma\left(\frac{9}{2}\right) = \left(\frac{9}{2} - 1\right)\Gamma\left(\frac{9}{2} - 1\right)$$

$$= \frac{7}{2}\Gamma\left(\frac{7}{2}\right)$$

$$= \frac{7}{2}\left(\frac{7}{2} - 1\right)\Gamma\left(\frac{7}{2} - 1\right)$$

$$= \frac{7}{2} \cdot \frac{5}{2} \cdot \Gamma\left(\frac{5}{2}\right) = \frac{35}{4} \cdot \frac{3}{2} \Gamma\left(\frac{3}{2}\right)$$

$$= \frac{105}{8} \cdot \frac{1}{2} \Gamma\left(\frac{1}{2}\right) = \frac{105}{16} \sqrt{\pi} //$$

6. (a). Expand $\log(1+x)$ by Maclaurin's series expansion.

Solⁿ: Let $f(x) = \log(1+x)$

$$f(0) = \log 1 = 0$$

$$f'(x) = \frac{1}{1+x}$$

$$f'(0) = \frac{1}{1+0} = 1$$

$$f''(x) = \frac{-1}{(1+x)^2}$$

$$f''(0) = \frac{-1}{1} = -1$$

$$\begin{aligned} f'''(x) &= (-1)(-2)(1+x)^{-3} \\ &= \frac{2}{(1+x)^3} \end{aligned}$$

$$f'''(0) = \frac{2}{(1+0)^3} = 2$$

$$\begin{aligned} f^{IV}(x) &= 2(-3)(1+x)^{-4} \\ &= \frac{-6}{(1+x)^4} \end{aligned}$$

$$f^{IV}(0) = \frac{-6}{(1+0)^4} = -6$$

by Maclaurin's series

$$f(x) = f(0) + xf'(0) + \frac{x^2}{2!} f''(0) + \frac{x^3}{3!} f'''(0) + \dots$$

$$\therefore f(x) = 0 + x(1) + \frac{x^2}{2!}(-1) + \frac{x^3}{3!}(2) + \frac{x^4}{4!}(-6) + \dots$$

$$= x - \frac{x^2}{2!} + \frac{x^3}{3} - \dots //$$

(b). obtain Taylor series expansion of e^x about

$$x: -1 \text{ (or)} x: 0 + 1.$$

Sol: Let $f(x) = e^x$

about $x = -1$

put $x+1 = t \Rightarrow x = t-1$

$$\therefore f(x) = e^x$$

$$= e^{t-1}$$

$$= e^t \cdot e^{-1} = \frac{e^t}{e} = \frac{1}{e} \left[1 + \frac{t}{1!} + \frac{t^2}{2!} + \frac{t^3}{3!} + \dots \right] \quad \because [t = x+1]$$

$$= \frac{1}{e} \left[1 + \frac{(x+1)}{1!} + \frac{(x+1)^2}{2!} + \frac{(x+1)^3}{3!} + \dots \right] //$$

7. (a). find 'c' for cauchy Mean value theorem for $f(x) = e^x$,

$$g(x) = e^{-x} \text{ in } [a, b].$$

Sol: Let $f(x) = e^x$, $g(x) = e^{-x}$ on $[a, b]$

$f(x)$ & $g(x)$ are continuous on $[a, b]$ &

$f(x)$, $g(x)$ are derivable on (a, b)

$$\text{also } g'(x) = -e^{-x} \neq 0$$

by cauchy Mean value theorem

$$\frac{f(b) - f(a)}{g(b) - g(a)} = \frac{f'(c)}{g'(c)} \rightarrow (1)$$

here

$$f(x) = e^x$$

$$f(a) = e^a$$

$$f(b) = e^b$$

$$\& f'(x) = e^x$$

$$g(x) = e^{-x}$$

$$g(a) = e^{-a}$$

$$g(b) = e^{-b}$$

$$\& g'(x) = -e^{-x}$$

from Eq (1)

$$\therefore \frac{e^b - e^a}{e^b - e^a} = \frac{e^c}{-e^c}$$

$$\Rightarrow \frac{e^b - e^a}{\frac{1}{e^b} - \frac{1}{e^a}} = \frac{-e^c}{\frac{1}{e^c}}$$

$$\Rightarrow \frac{e^b - e^a}{\frac{e^a - e^b}{e^a \cdot e^b}} = -e^c \cdot e^c$$

$$\Rightarrow -e^{a+b} = -e^{c+c}$$

$$\Rightarrow a+b = 2c \Rightarrow \boxed{c = \frac{a+b}{2}}$$

(b). obtain Taylor series expansion of $\sin x$ in powers of $x - \frac{\pi}{4}$.

Sol: Let $f(x) = \sin x$ at $a = \pi/4$

here

$$f'(x) = \cos x$$

$$f''(x) = -\sin x$$

$$f'''(x) = -\cos x$$

$$f^{IV}(x) = \sin x$$

$$f(\pi/4) = \sin \pi/4 = 1/\sqrt{2}$$

$$f'(\pi/4) = \cos \pi/4 = 1/\sqrt{2}$$

$$f''(\pi/4) = -\sin \pi/4 = -1/\sqrt{2}$$

$$f'''(\pi/4) = -\cos \pi/4 = -1/\sqrt{2}$$

$$f^{IV}(\pi/4) = \sin \pi/4 = 1/2$$

by Taylor series

$$f(x) = f(a) + (x-a)f'(a) + \frac{(x-a)^2}{2!}f''(a) + \frac{(x-a)^3}{3!}f'''(a) + \dots$$

$$= \frac{1}{\sqrt{2}} + (x - \frac{\pi}{4})\frac{1}{\sqrt{2}} + \frac{1}{2!}(x - \frac{\pi}{4})^2\left(\frac{-1}{\sqrt{2}}\right) + \frac{1}{3!}(x - \frac{\pi}{4})^3\left(\frac{-1}{\sqrt{2}}\right) + \dots$$

$$= \frac{1}{\sqrt{2}} \left[1 + (x - \frac{\pi}{4}) - \frac{1}{2!}(x - \frac{\pi}{4})^2 - \frac{1}{3!}(x - \frac{\pi}{4})^3 + \dots \right]$$

8. If $x = r \sin \theta \cos \phi$, $y = r \sin \theta \sin \phi$, $z = r \cos \theta$ then show that $\frac{\partial(x, y, z)}{\partial(r, \theta, \phi)} = r^2 \sin \theta$.

Given

$$x = r \sin \theta \cos \phi$$

$$y = r \sin \theta \sin \phi$$

$$z = r \cos \theta$$

now,

$$\frac{\partial x}{\partial r} = \sin \theta \cos \phi \quad (1)$$

$$\frac{\partial y}{\partial r} = \sin \theta \sin \phi \quad (2)$$

$$\frac{\partial z}{\partial r} = \cos \theta \quad (3)$$

$$\frac{\partial x}{\partial \theta} = r \cos \phi \cdot \cos \theta$$

$$\frac{\partial y}{\partial \theta} = r \sin \phi \cdot \cos \theta$$

$$\frac{\partial z}{\partial \theta} = r \cdot (-\sin \theta) = -r \sin \theta$$

$$\frac{\partial x}{\partial \phi} = r \sin \theta \cdot (-\sin \phi)$$

$$\frac{\partial y}{\partial \phi} = r \sin \theta \cdot \cos \phi$$

$$\frac{\partial z}{\partial \phi} = 0$$

consider $\frac{\partial(x, y, z)}{\partial(r, \theta, \phi)}$

$$= \begin{vmatrix} \frac{\partial x}{\partial r} & \frac{\partial x}{\partial \theta} & \frac{\partial x}{\partial \phi} \\ \frac{\partial y}{\partial r} & \frac{\partial y}{\partial \theta} & \frac{\partial y}{\partial \phi} \\ \frac{\partial z}{\partial r} & \frac{\partial z}{\partial \theta} & \frac{\partial z}{\partial \phi} \end{vmatrix} = \begin{vmatrix} \sin \theta \cos \phi & r \cos \phi \cos \theta & -r \sin \theta \sin \phi \\ \sin \theta \sin \phi & r \sin \phi \cos \theta & r \sin \theta \cos \phi \\ \cos \theta & -r \sin \theta & 0 \end{vmatrix}$$

$$= \sin \theta \cos \phi [0 + r^2 \sin^2 \theta \cos \phi] - r \cos \phi \cos \theta [0 - r \sin \theta \cos \theta \cos \phi]$$

$$- r \sin \theta \sin \phi [-r \sin^2 \theta \sin \phi - r \sin \phi \cos^2 \theta]$$

$$= r^2 \sin^3 \theta \cos^2 \phi + r^2 \sin \theta \cos^2 \theta \cdot \cos^2 \phi + r^2 \sin^3 \theta \sin^2 \phi + r^2 \sin \theta \sin^2 \phi \cos^2 \theta$$

$$= r^2 \sin \theta \cos^2 \phi [\sin^2 \theta + \cos^2 \theta] + r^2 \sin \theta \sin^2 \phi [\sin^2 \theta + \cos^2 \theta]$$

$$= r^2 \sin \theta \cos^2 \phi (1) + r^2 \sin \theta \sin^2 \phi (1)$$

$$= r^2 \sin \theta [\sin^2 \phi + \cos^2 \phi]$$

$$= r^2 \sin \theta (1) = r^2 \sin \theta \quad //$$

9). find the dimension of the rectangular box, when top is opened volume is 108 cubic

9/A)

Let x, y, z be the dimensions of a rectangular parallelepiped opened at top

$$V = xyz$$

given $V = 108$ cubic feet.

$$xyz = 108$$

$$\Rightarrow xyz - 108 = 0 \rightarrow (1)$$

here $\phi(x, y, z) = xyz - 108$

$$S = xy + 2yz + 2zx$$

Let $f(x, y, z) = xy + 2yz + 2zx \rightarrow (2)$

$$\begin{aligned} F(x, y, z) &= f(x, y, z) + \lambda \phi(x, y, z) \\ &= xy + 2yz + 2zx + \lambda(xyz - 108) \\ &= xy + 2yz + 2zx + \lambda xyz - \lambda 108 \end{aligned}$$

now, $\frac{\partial F}{\partial x} = y + 2z + \lambda yz$

$$\frac{\partial F}{\partial y} = x + 2z + \lambda xz$$

$$\frac{\partial F}{\partial z} = 2y + 2x + \lambda xy$$

$$\therefore \frac{\partial F}{\partial x} = 0$$

$$\frac{\partial F}{\partial y} = 0$$

$$\frac{\partial F}{\partial z} = 0$$

$$\Rightarrow y + 2z + \lambda yz = 0$$

$$\Rightarrow x + 2z + \lambda xz = 0$$

$$\Rightarrow 2y + 2x + \lambda xy = 0$$

$$\Rightarrow \lambda yz = -(y + 2z)$$

$$\Rightarrow \lambda xz = -(x + 2z)$$

$$\Rightarrow \lambda xy = -(2y + 2x)$$

$$\Rightarrow \lambda = \frac{-(y + 2z)}{yz}$$

$$\Rightarrow \lambda = \frac{-(x + 2z)}{xz}$$

$$\Rightarrow \lambda = \frac{-(2y + 2x)}{xy}$$

consider

$$\frac{-(y + 2z)}{yz} = \frac{-(x + 2z)}{xz}$$

$$\& \quad \frac{-(x + 2z)}{xz} = \frac{-(2y + 2x)}{xy}$$

$$\Rightarrow xy + 2xz = xy + 2yz$$

$$y(x + 2z) = z(2y + 2x)$$

$$\Rightarrow 2xz = 2yz$$

$$xy + 2yz = 2yz + 2xz$$

$$xy = 2xz$$

$$\Rightarrow \boxed{x = y}$$

$$\Rightarrow \boxed{y = 2z}$$

$$\therefore x = y = 2z$$

now, $xyz = 108$

$$\therefore \begin{cases} y = x \\ z = x/2 \end{cases}$$

$$\Rightarrow x(x)\left(\frac{x}{2}\right) = 108$$

$$\Rightarrow x^3 = (108) 2$$

$$\Rightarrow x^3 = 216$$

$$\Rightarrow x^3 = 6^3$$

$$\Rightarrow \boxed{x = 6}$$

$$\therefore y = 6 \quad \& \quad z = \frac{x}{2} = \frac{6}{2} = 3$$

dimensions are $x = 6, y = 6, z = 3$. //

10). Relation between beta & Gamma function

$$\beta(m, n) = \frac{\Gamma(m) \Gamma(n)}{\Gamma(m+n)}$$

Proof: consider

$$\Gamma(m) = \int_0^{\infty} e^{-x} \cdot x^{m-1} dx$$

$$\text{put } x = yt$$

$$dx = y dt$$

$$\therefore \int_0^{\infty} e^{-yt} \cdot (yt)^{m-1} y dt$$

$$\Rightarrow \Gamma(m) = \int_0^{\infty} e^{-yt} \cdot y^{m-1} \cdot t^{m-1} y dt$$
$$= \int_0^{\infty} e^{-yt} \cdot y^m t^{m-1} dt$$

$$\Rightarrow \frac{\Gamma(m)}{y^m} = \int_0^{\infty} e^{-yt} \cdot t^{m-1} dt$$

multiply $\int_0^{\infty} e^{-y} \cdot y^{m+n-1} dy$ on both sides

$$\Rightarrow \int_0^{\infty} \frac{\Gamma(m)}{y^m} \cdot e^{-y} \cdot y^{m+n-1} dy = \int_0^{\infty} \int_0^{\infty} e^{-yx} \cdot e^{-y} \cdot y^{m+n-1} dy \cdot x^{m-1} dx$$

$$\Rightarrow \Gamma(m) \int_0^{\infty} e^{-y} \cdot y^{n-1} dy = \int_0^{\infty} \int_0^{\infty} e^{-y(x+1)} \cdot y^{m+n-1} dy \cdot x^{m-1} dx$$

$$\Rightarrow \Gamma(m) \cdot \Gamma(n) = \int_0^\infty \frac{\Gamma(m+n)}{(x+1)^{m+n}} \cdot x^{m-1} dx \quad \because \Gamma(n) = \int_0^\infty e^{-x} \cdot x^{n-1} dx \quad (9)$$

$$= \Gamma(m+n) \int_0^\infty \frac{x^{m-1}}{(x+1)^{m+n}} dx$$

$$= \Gamma(m+n) B(m, n)$$

$$\Rightarrow \boxed{B(m, n) = \frac{\Gamma(m) \cdot \Gamma(n)}{\Gamma(m+n)}}$$

11. Evaluate $\int_0^1 \int_0^{\sqrt{1+x^2}} \frac{dy dx}{1+x^2+y^2}$

Sol: Given integral

$$I = \int_{x=0}^1 \left[\int_{y=0}^{\sqrt{1+x^2}} \frac{dy}{1+x^2+y^2} \right] dx$$

$$= \int_{x=0}^1 \int_{y=0}^{\sqrt{1+x^2}} \frac{dy}{\left[\frac{\sqrt{1+x^2}}{a^2} \right]^2 + y^2} dx$$

$$\therefore \int \frac{1}{a^2+x^2} dx = \frac{1}{a} \tan^{-1} \frac{x}{a}$$

$$= \int_{x=0}^1 \frac{1}{\sqrt{1+x^2}} \left[\tan^{-1} \frac{y}{\frac{\sqrt{1+x^2}}{a^2}} \right]_{y=0}^{\sqrt{1+x^2}} dx$$

$$= \int_{x=0}^1 \frac{1}{\sqrt{1+x^2}} \left[\tan^{-1} \frac{\sqrt{1+x^2}}{\frac{\sqrt{1+x^2}}{a^2}} - \tan^{-1} 0 \right] dx$$

$$= \int_{x=0}^1 \frac{1}{\sqrt{1+x^2}} \left[\tan^{-1}(1) - 0 \right] dx$$

$$= \int_{x=0}^1 \frac{1}{\sqrt{1+x^2}} \tan^{-1}(\tan \frac{\pi}{4}) dx = \frac{\pi}{4} \int_0^1 \frac{1}{\sqrt{1+x^2}} dx$$

$$= \frac{\pi}{4} \log [x + \sqrt{x^2+1}]_0^1$$

$$= \frac{\pi}{4} [\log(1 + \sqrt{1+1}) - \log(0 + \sqrt{0+1})] = \frac{\pi}{4} \log(1 + \sqrt{2}) - 0$$

$$= \frac{\pi}{4} \log(1 + \sqrt{2}) //$$

Q. Evaluate $\int_{-1}^1 \int_0^z \int_{x-z}^{x+z} (x+y+z) dx dy dz$.

sol: Given Integral

$$I = \int_{-1}^1 \int_0^z \int_{x-z}^{x+z} (x+y+z) dx dy dz$$

$$= \int_{-1}^1 \int_0^z \left[(x+z)(y) + \frac{y^2}{2} \right]_{x-z}^{x+z} dx dz$$

$$= \int_{-1}^1 \int_0^z \left[(x+z)[x+z-x+z] + \frac{1}{2} [(x+z)^2 - (x-z)^2] \right] dx dz$$

$$= \int_{-1}^1 \int_0^z \left[(x+z)(2z) + \frac{1}{2} (4xz) \right] dx dz$$

$$= 2 \int_{-1}^1 \int_0^z (xz + z^2 + xz) dx dz$$

$$= 2 \int_{-1}^1 \int_0^z (2xz + z^2) dx dz = 2 \int_{-1}^1 \left(2z \frac{x^2}{2} + xz^2 \right)_0^z dz$$

$$= 2 \int_{-1}^1 [z(z^2) + \cancel{x}z^2] - 0 dz$$

$$= 2 \int_{-1}^1 2z^3 dz = 4 \left(\frac{z^4}{4} \right)_{-1}^1$$

$$= 1 - (-1)^4$$

$$= 0 //$$

Q. Evaluate: $\int_0^1 \int_0^x x dy dx$

$$= \int_0^1 x(y)_0^x dx$$

$$= \int_0^1 x(x-0) dx = \int_0^1 x^2 dx = \left(\frac{x^3}{3} \right)_0^1 = \frac{1}{3} - 0 = \frac{1}{3} //$$